format-version: 1.0
data-version: 1
date: 05:23:2016 03:00
saved-by: sgn
default-namespace: musa_time_ontology
remark: none
ontology: musa_time

[Term]
id: MUSATIME:0000000
name: musa_time_terms

[Term]
id: MUSATIME:0000001
name: time of day
def: "Categorical day periods." []
is_a: MUSATIME:0000000

[Term]
id: MUSATIME:0000002
name: end of night
synonym: "EoN" EXACT []
def: "Half an hour before sunrise." []
is_a: MUSATIME:0000001

[Term]
id: MUSATIME:0000003
name: end of day
synonym: "EoD" EXACT []
def: "Late afternoon daylight." []
is_a: MUSATIME:0000001

[Term]
id: MUSATIME:0000004
name: mid day
synonym: "MD" EXACT []
def: "Between 11:00 in the morning and 14:00 in the afternoon." []
is_a: MUSATIME:0000001

[Term]
id: MUSATIME:0000005
name: time of year
def: "Weeks and months." []
is_a: MUSATIME:0000000

[Term]
id: MUSATIME:0000006
name: week 1
synonym: "Wk1" EXACT []
def: "" []
is_a: MUSATIME:0000005

[Term]
id: MUSATIME:0000007
name: week 2
synonym: "Wk2" EXACT []
def: "" []
is_a: MUSATIME:0000005

[Term]
id: MUSATIME:0000008
name: week 3
synonym: "Wk3" EXACT []
def: "" []
is_a: MUSATIME:0000005

[Term]
id: MUSATIME:0000009
name: week 4
synonym: "Wk4" EXACT []
def: "" []
is_a: MUSATIME:0000005

[Term]
id: MUSATIME:0000010
name: week 5
synonym: "Wk5" EXACT []
def: "" []
is_a: MUSATIME:0000005

[Term]
id: MUSATIME:0000011
name: week 6
synonym: "Wk6" EXACT []
def: "" []
is_a: MUSATIME:0000005

[Term]
id: MUSATIME:0000012
name: week 7
synonym: "Wk7" EXACT []
def: "" []
is_a: MUSATIME:0000005

[Term]
id: MUSATIME:0000013
name: week 8
synonym: "Wk8" EXACT []
def: "" []
is_a: MUSATIME:0000005

[Term]
id: MUSATIME:0000014
name: week 9
synonym: "Wk9" EXACT []
def: "" []
is_a: MUSATIME:0000005

[Term]
id: MUSATIME:0000015
name: week 10
synonym: "Wk10" EXACT []
def: "" []
is_a: MUSATIME:0000005

[Term]
id: MUSATIME:0000016
name: week 11
synonym: "Wk11" EXACT []
def: "" []
is_a: MUSATIME:0000005

[Term]
id: MUSATIME:0000017
name: week 12
synonym: "Wk12" EXACT []
def: "" []
is_a: MUSATIME:0000005

[Term]
id: MUSATIME:0000018
name: week 13
synonym: "Wk13" EXACT []
def: "" []
is_a: MUSATIME:0000005

[Term]
id: MUSATIME:0000019
name: week 14
synonym: "Wk14" EXACT []
def: "" []
is_a: MUSATIME:0000005

[Term]
id: MUSATIME:0000020
name: week 15
synonym: "Wk15" EXACT []
def: "" []
is_a: MUSATIME:0000005

[Term]
id: MUSATIME:0000021
name: week 16
synonym: "Wk16" EXACT []
def: "" []
is_a: MUSATIME:0000005

[Term]
id: MUSATIME:0000022
name: week 17
synonym: "Wk17" EXACT []
def: "" []
is_a: MUSATIME:0000005

[Term]
id: MUSATIME:0000023
name: week 18
synonym: "Wk18" EXACT []
def: "" []
is_a: MUSATIME:0000005

[Term]
id: MUSATIME:0000024
name: week 19
synonym: "Wk19" EXACT []
def: "" []
is_a: MUSATIME:0000005

[Term]
id: MUSATIME:0000025
name: week 20
synonym: "Wk20" EXACT []
def: "" []
is_a: MUSATIME:0000005

[Term]
id: MUSATIME:0000026
name: week 21
synonym: "Wk21" EXACT []
def: "" []
is_a: MUSATIME:0000005

[Term]
id: MUSATIME:0000027
name: week 22
synonym: "Wk22" EXACT []
def: "" []
is_a: MUSATIME:0000005

[Term]
id: MUSATIME:0000028
name: week 23
synonym: "Wk23" EXACT []
def: "" []
is_a: MUSATIME:0000005

[Term]
id: MUSATIME:0000029
name: week 24
synonym: "Wk24" EXACT []
def: "" []
is_a: MUSATIME:0000005

[Term]
id: MUSATIME:0000030
name: week 25
synonym: "Wk25" EXACT []
def: "" []
is_a: MUSATIME:0000005

[Term]
id: MUSATIME:0000031
name: week 26
synonym: "Wk26" EXACT []
def: "" []
is_a: MUSATIME:0000005

[Term]
id: MUSATIME:0000032
name: week 27
synonym: "Wk27" EXACT []
def: "" []
is_a: MUSATIME:0000005

[Term]
id: MUSATIME:0000033
name: week 28
synonym: "Wk28" EXACT []
def: "" []
is_a: MUSATIME:0000005

[Term]
id: MUSATIME:0000034
name: week 29
synonym: "Wk29" EXACT []
def: "" []
is_a: MUSATIME:0000005

[Term]
id: MUSATIME:0000035
name: week 30
synonym: "Wk30" EXACT []
def: "" []
is_a: MUSATIME:0000005

[Term]
id: MUSATIME:0000036
name: week 31
synonym: "Wk31" EXACT []
def: "" []
is_a: MUSATIME:0000005

[Term]
id: MUSATIME:0000037
name: week 32
synonym: "Wk32" EXACT []
def: "" []
is_a: MUSATIME:0000005

[Term]
id: MUSATIME:0000038
name: week 33
synonym: "Wk33" EXACT []
def: "" []
is_a: MUSATIME:0000005

[Term]
id: MUSATIME:0000039
name: week 34
synonym: "Wk34" EXACT []
def: "" []
is_a: MUSATIME:0000005

[Term]
id: MUSATIME:0000040
name: week 35
synonym: "Wk35" EXACT []
def: "" []
is_a: MUSATIME:0000005

[Term]
id: MUSATIME:0000041
name: week 36
synonym: "Wk36" EXACT []
def: "" []
is_a: MUSATIME:0000005

[Term]
id: MUSATIME:0000042
name: week 37
synonym: "Wk37" EXACT []
def: "" []
is_a: MUSATIME:0000005

[Term]
id: MUSATIME:0000043
name: week 38
synonym: "Wk38" EXACT []
def: "" []
is_a: MUSATIME:0000005

[Term]
id: MUSATIME:0000044
name: week 39
synonym: "Wk39" EXACT []
def: "" []
is_a: MUSATIME:0000005

[Term]
id: MUSATIME:0000045
name: week 40
synonym: "Wk40" EXACT []
def: "" []
is_a: MUSATIME:0000005

[Term]
id: MUSATIME:0000046
name: week 41
synonym: "Wk41" EXACT []
def: "" []
is_a: MUSATIME:0000005

[Term]
id: MUSATIME:0000047
name: week 42
synonym: "Wk42" EXACT []
def: "" []
is_a: MUSATIME:0000005

[Term]
id: MUSATIME:0000048
name: week 43
synonym: "Wk43" EXACT []
def: "" []
is_a: MUSATIME:0000005

[Term]
id: MUSATIME:0000049
name: week 44
synonym: "Wk44" EXACT []
def: "" []
is_a: MUSATIME:0000005

[Term]
id: MUSATIME:0000050
name: week 45
synonym: "Wk45" EXACT []
def: "" []
is_a: MUSATIME:0000005

[Term]
id: MUSATIME:0000051
name: week 46
synonym: "Wk46" EXACT []
def: "" []
is_a: MUSATIME:0000005

[Term]
id: MUSATIME:0000052
name: week 47
synonym: "Wk47" EXACT []
def: "" []
is_a: MUSATIME:0000005

[Term]
id: MUSATIME:0000053
name: week 48
synonym: "Wk48" EXACT []
def: "" []
is_a: MUSATIME:0000005

[Term]
id: MUSATIME:0000054
name: week 49
synonym: "Wk49" EXACT []
def: "" []
is_a: MUSATIME:0000005

[Term]
id: MUSATIME:0000055
name: week 50
synonym: "Wk50" EXACT []
def: "" []
is_a: MUSATIME:0000005

[Term]
id: MUSATIME:0000056
name: week 51
synonym: "Wk51" EXACT []
def: "" []
is_a: MUSATIME:0000005

[Term]
id: MUSATIME:0000057
name: week 52
synonym: "Wk52" EXACT []
def: "" []
is_a: MUSATIME:0000005

[Term]
id: MUSATIME:0000058
name: week 53
synonym: "Wk53" EXACT []
def: "" []
is_a: MUSATIME:0000005

[Term]
id: MUSATIME:0000059
name: week 54
synonym: "Wk54" EXACT []
def: "" []
is_a: MUSATIME:0000005

[Term]
id: MUSATIME:0000060
name: month 1
synonym: "Mo1" EXACT []
def: "" []
is_a: MUSATIME:0000005

[Term]
id: MUSATIME:0000061
name: month 2
synonym: "Mo2" EXACT []
def: "" []
is_a: MUSATIME:0000005

[Term]
id: MUSATIME:0000062
name: month 3
synonym: "Mo3" EXACT []
def: "" []
is_a: MUSATIME:0000005

[Term]
id: MUSATIME:0000063
name: month 4
synonym: "Mo4" EXACT []
def: "" []
is_a: MUSATIME:0000005

[Term]
id: MUSATIME:0000064
name: month 5
synonym: "Mo5" EXACT []
def: "" []
is_a: MUSATIME:0000005

[Term]
id: MUSATIME:0000065
name: month 6
synonym: "Mo6" EXACT []
def: "" []
is_a: MUSATIME:0000005

[Term]
id: MUSATIME:0000066
name: month 7
synonym: "Mo7" EXACT []
def: "" []
is_a: MUSATIME:0000005

[Term]
id: MUSATIME:0000067
name: month 8
synonym: "Mo8" EXACT []
def: "" []
is_a: MUSATIME:0000005

[Term]
id: MUSATIME:0000068
name: month 9
synonym: "Mo9" EXACT []
def: "" []
is_a: MUSATIME:0000005

[Term]
id: MUSATIME:0000069
name: month 10
synonym: "Mo10" EXACT []
def: "" []
is_a: MUSATIME:0000005

[Term]
id: MUSATIME:0000070
name: month 11
synonym: "Mo11" EXACT []
def: "" []
is_a: MUSATIME:0000005

[Term]
id: MUSATIME:0000071
name: month 12
synonym: "Mo12" EXACT []
def: "" []
is_a: MUSATIME:0000005

[Term]
id: MUSATIME:0000072
name: time of generation
def: "Categorical plant generations." []
is_a: MUSATIME:0000000

[Term]
id: MUSATIME:0000073
name: cycle 1
synonym: "C1" EXACT []
def: "First cycle (or ratoon one)." []
is_a: MUSATIME:0000072

[Term]
id: MUSATIME:0000074
name: cycle 2
synonym: "C2" EXACT []
def: "Second cycle (or ratoon two)." []
is_a: MUSATIME:0000072

[Term]
id: MUSATIME:0000075
name: cycle 3
synonym: "C3" EXACT []
def: "Third cycle (or ratoon three)." []
is_a: MUSATIME:0000072

[Term]
id: MUSATIME:0000076
name: cycle 4
synonym: "C4" EXACT []
def: "Fourth cycle (or ratoon four)." []
is_a: MUSATIME:0000072

[Term]
id: MUSATIME:0000077
name: cycle 5
synonym: "C5" EXACT []
def: "Fifth cycle (or ratoon five)." []
is_a: MUSATIME:0000072

[Term]
id: MUSATIME:0000078
name: cycle 6
synonym: "C6" EXACT []
def: "Sixth cycle (or ratoon six)." []
is_a: MUSATIME:0000072

id: MUSATIME:0000079
name: time of data collection
def: "Growing stages at which data is collected" []
is_a: MUSATIME:0000000

[Term]
id: MUSATIME:0000080
name: shooting stage
synonym: "shooting" EXACT []
def: "shooting stage." []
is_a: MUSATIME:0000079

[Term]
id: MUSATIME:0000081
name: planting stage
synonym: "planting" EXACT []
def: "planting stage." []
is_a: MUSATIME:0000079

[Term]
id: MUSATIME:0000082
name: harvesting stage
synonym: "harvest" EXACT []
def: "harvesting stage." []
is_a: MUSATIME:0000079

[Term]
id: MUSATIME:0000083
name: postharvest stage
synonym: "p-harvest" EXACT []
def: "postharvesting stage." []
is_a: MUSATIME:0000079